a

reduction_directedHamiltonianCircuit_to_hamiltonianCircuit/left_lemma_working_file.dfy
@@ -46,35 +46,35 @@ module LeftLemma
         ensures forall i :: 0<=i<|c| ==> isUndirectedHamiltonianCircuit(g, cicle_sequence(c, i))
     {}
 
-    ghost predicate in_out_circuit(g: Graph, uc: seq<nat>)
+    ghost predicate in_out_circuit(g: Graph, c: seq<nat>)
         requires validUndirectedGraph(g)
         requires |g|>2 && |g|%3==0
         requires in_out_graph(g)
         // requires isUndirectedHamiltonianCircuit(g, uc)
     {
-        isUndirectedHamiltonianCircuit(g, uc)
+        isUndirectedHamiltonianCircuit(g, c)
         &&
-        forall i :: 0<i<|uc|-1 ==>
+        forall i :: 0<i<|c|-1 ==>
         (
-            (0<=uc[i]<|g|/3 ==>  //case og node
+            (0<=c[i]<|g|/3 ==>  //case og node
             (
-                uc[i-1]==uc[i]+(|g|/3)*2  //before: in
+                c[i-1]==c[i]+(|g|/3)*2  //before: in
                 &&
-                uc[i+1]==uc[i]+|g|/3    //next: out
+                c[i+1]==c[i]+|g|/3    //next: out
             ))
             &&
-            (|g|/3<=uc[i]<(|g|/3)*2 ==>  //case out node
+            (|g|/3<=c[i]<(|g|/3)*2 ==>  //case out node
             (
-                uc[i-1]==uc[i]-|g|/3   //before: og
+                c[i-1]==c[i]-|g|/3   //before: og
                 &&
-                (|g|/3)*2<=uc[i+1]<|g|   //next: in (range)
+                (|g|/3)*2<=c[i+1]<|g|   //next: in (range)
             ))
             &&
-            ((|g|/3)*2<=uc[i]<|g| ==>  //case in node
+            ((|g|/3)*2<=c[i]<|g| ==>  //case in node
             (
-                |g|/3<=uc[i-1]<(|g|/3)*2   //before: out (range)
+                |g|/3<=c[i-1]<(|g|/3)*2   //before: out (range)
                 &&
-                uc[i+1]==uc[i]-(|g|/3)*2    //next: og
+                c[i+1]==c[i]-(|g|/3)*2    //next: og
             ))
         )
     }
@@ -86,8 +86,89 @@ module LeftLemma
         requires in_out_graph(g)
         ensures in_out_circuit(g, c)
     {
-        
+        forall i | 0<i<|c|-1
+        {
+            in_out_circuit_local_lemma(g, c, i);
+        }
     }
+
+    lemma in_out_circuit_local_lemma(g: Graph, c: seq<nat>, i: int)
+        requires validUndirectedGraph(g)
+        requires |g|>2 && |g|%3==0
+        requires isUndirectedHamiltonianCircuit(g, c)
+        requires in_out_graph(g)
+        requires 0<i<|c|-1
+        ensures
+        (
+            (0<=c[i]<|g|/3 ==>  //case og node
+            (
+                c[i-1]==c[i]+(|g|/3)*2  //before: in
+                &&
+                c[i+1]==c[i]+|g|/3    //next: out
+            ))
+            &&
+            (|g|/3<=c[i]<(|g|/3)*2 ==>  //case out node
+            (
+                c[i-1]==c[i]-|g|/3   //before: og
+                &&
+                (|g|/3)*2<=c[i+1]<|g|   //next: in (range)
+            ))
+            &&
+            ((|g|/3)*2<=c[i]<|g| ==>  //case in node
+            (
+                |g|/3<=c[i-1]<(|g|/3)*2   //before: out (range)
+                &&
+                c[i+1]==c[i]-(|g|/3)*2    //next: og
+            ))
+        )
+    {
+        if 0<=c[i]<|g|/3
+        {
+            in_out_circuit_1_lemma(g, c, i);
+        }
+        if |g|/3<=c[i]<(|g|/3)*2
+        {
+            in_out_circuit_2_lemma(g, c, i);
+        }
+        if (|g|/3)*2<=c[i]<|g|
+        {
+            in_out_circuit_3_lemma(g, c, i);
+        }
+    }
+
+
+    lemma in_out_circuit_1_lemma(g: Graph, c: seq<nat>, i: int)
+        requires validUndirectedGraph(g)
+        requires |g|>2 && |g|%3==0
+        requires isUndirectedHamiltonianCircuit(g, c)
+        requires in_out_graph(g)
+        requires 0<i<|c|-1
+        requires 0<=c[i]<|g|/3
+        ensures c[i-1]==c[i]+(|g|/3)*2 && c[i+1]==c[i]+|g|/3
+    {}
+    
+    lemma in_out_circuit_2_lemma(g: Graph, c: seq<nat>, i: int)
+        requires validUndirectedGraph(g)
+        requires |g|>2 && |g|%3==0
+        requires isUndirectedHamiltonianCircuit(g, c)
+        requires in_out_graph(g)
+        requires 0<i<|c|-1
+        requires |g|/3<=c[i]<(|g|/3)*2
+        ensures c[i-1]==c[i]-|g|/3 && (|g|/3)*2<=c[i+1]<|g|
+    {}
+
+    lemma in_out_circuit_3_lemma(g: Graph, c: seq<nat>, i: int)
+        requires validUndirectedGraph(g)
+        requires |g|>2 && |g|%3==0
+        requires isUndirectedHamiltonianCircuit(g, c)
+        requires in_out_graph(g)
+        requires 0<i<|c|-1
+        requires (|g|/3)*2<=c[i]<|g|
+        ensures |g|/3<=c[i-1]<(|g|/3)*2 && c[i+1]==c[i]-(|g|/3)*2 
+    {}
+
+
+
 
     //starts with in_node -> og_node -> out_node ...and so on...
     ghost predicate in_out_circuit_std(g: Graph, uc: seq<nat>)
